Add symbolic and numeric derivatives

ListAdd.v
@@ -46,4 +46,34 @@ Section incl.
         + exists a; intuition.
     Qed.
 
-End incl.
+    End incl.
+
+Section olist.
+  
+  Fixpoint listo_to_olist {a: Type} (l: list (option a)) : option (list a) :=
+    match l with
+    | nil => Some nil
+    | Some x :: xs => match listo_to_olist xs with
+                      | None => None
+                      | Some xs => Some (x::xs)
+                      end
+    | None :: xs => None
+    end.
+  
+  Lemma listo_to_olist_some {A:Type} (l:list (option A)) (l':list A) :
+      listo_to_olist l = Some l' ->
+      l = (map Some l').
+    Proof.
+      revert l'.
+      induction l; simpl; intros l' eqq.
+      - inversion eqq; subst; simpl; trivial.
+      - destruct a; try discriminate.
+        case_eq (listo_to_olist l)
+        ; [intros ? eqq2 | intros eqq2]
+        ; rewrite eqq2 in eqq
+        ; try discriminate.
+        inversion eqq; subst.
+        rewrite (IHl l0); trivial. 
+    Qed.
+
+End olist.
